compiler/dsl/coq/ReflexEcho.v
@@ -20,7 +20,7 @@ Definition PAYD : vvdesc NB_MSG := mk_vvdesc
 
 Notation M := 0%fin (only parsing).
 
-Inductive COMPT' : Type := Echo.
+Inductive COMPT' : Type := Echo1 | Echo2.
 Definition COMPT := COMPT'.
 
 Definition COMPTDEC : forall (x y : COMPT), decide (x = y).
@@ -28,13 +28,15 @@ Proof. decide equality. Defined.
 
 Definition COMPS (t : COMPT) : compd :=
   match t with
-  | Echo => mk_compd "Echo" "test/echo-00/test.py" [] (mk_vdesc [])
+  | Echo1 => mk_compd "Echo" "test/echo-00/test.py" [] (mk_vdesc [])
+  | Echo2 => mk_compd "Echo" "test/echo-00/test.py" [] (mk_vdesc [])
   end.
 
 Definition KSTD : vcdesc COMPT := mk_vcdesc [].
 
 Definition IENVD : vcdesc COMPT := mk_vcdesc
-  [ Comp _ Echo
+  [ Comp _ Echo1;
+    Comp _ Echo2
   ].
 
 End SystemFeatures.
@@ -50,12 +52,12 @@ Module Spec <: SpecInterface.
 Include SystemFeatures.
 
 Definition INIT : init_prog PAYD COMPT COMPS KSTD IENVD :=
-  seq (spawn IENVD _ Echo tt None (Logic.eq_refl _))
-  nop.
+  seq (spawn IENVD _ Echo1 tt None (Logic.eq_refl _))
+  (seq (spawn IENVD _ Echo2 tt (Some None) (Logic.eq_refl _))
+  nop).
 
 Definition HANDLERS : handlers PAYD COMPT COMPS KSTD :=
   fun m cc =>
-    let (_, cf, _) := cc in
     match m as _m return forall (EQ : _m = m), _ with
     | Build_msg None p => fun EQ =>
       let envd := existT _ 0 tt in
@@ -68,6 +70,212 @@ Definition HANDLERS : handlers PAYD COMPT COMPS KSTD :=
       match bad with end
     end (Logic.eq_refl m).
 
+Require Import NonInterference.
+
+Require Import Ynot.
+
+Ltac destruct_fin f :=
+  match type of f with
+  | False => destruct f
+  | _ => let f' := fresh "f" in
+         destruct f as [ f' | ]; [destruct_fin f' | ]
+  end.
+
+Ltac destruct_pay pay :=
+  compute in pay;
+  match type of pay with
+  | unit => idtac
+  | _ => let a := fresh "a" in
+         let b := fresh "b" in
+         destruct pay as [a b]; simpl in a; destruct_pay b
+  end.
+
+Ltac destruct_msg :=
+  match goal with
+  | [ m : msg _ |- _ ]
+      => let tag := fresh "tag" in
+         let pay := fresh "pay" in
+         destruct m as [tag pay]; destruct_fin tag;
+         destruct_pay pay
+  end.
+
+(*Destructs num, str, or fd equalities in the context.*)
+Ltac destruct_eq H :=
+  repeat match type of H with
+         | context[if ?x then _ else _ ]
+           => destruct x
+         end.
+ (* repeat match type of H with
+         | context[num_eq ?a ?b]
+           => destruct (num_eq a b); simpl in *
+         | context[str_eq ?a ?b]
+           => destruct (str_eq a b); simpl in *
+         | context[fd_eq ?a ?b]
+           => destruct (fd_eq a b); simpl in *
+         end.*)
+
+Ltac destruct_input input :=
+  simpl in input; (*compute in input;*)
+  match type of input with
+  | unit => idtac
+  | _ => let x := fresh "x" in
+         let input' := fresh "input'" in
+         destruct input as [x input']; destruct_input input'
+  end.
+
+Ltac unpack_inhabited :=
+  repeat match goal with
+         | [ H : ktr _ _ _ _ _ = inhabits ?tr |- _ ]
+           => simpl in H; apply pack_injective in H; subst tr
+         end.
+
+Ltac unpack :=
+  match goal with
+  (*Valid exchange.*)
+  | [ s : Reflex.kstate _ _ _ _, s' : Reflex.kstate _ _ _ _ |- _ ]
+    => match goal with
+       | [ _ : kstate_run_prog _ _ _ _ _ _ _ _ s _ = s' |- _ ]
+         => subst s; subst s'
+       end
+  (*Initialization.*)
+  | [ s : Reflex.init_state _ _ _ _ _ |- _ ]
+    => match goal with
+         | [ H : s = Reflex.init_state_run_cmd _ _ _ _ _ _ _ _ |- _ ]
+           => subst s
+       end
+  (*Bogus msg*)
+  end; unpack_inhabited.
+
+Definition labeler (c : comp COMPT COMPS) :=
+  match comp_type _ _ c with
+  | Echo1 => true
+  | Echo2 => false
+  end.
+
+Local Opaque str_of_string.
+
+Ltac spawn_call :=
+      match goal with
+      | [ Hcall : call_ok _ _ _ _ _ _ |- call_ok _ _ _ _ _ _ ]
+          => repeat apply call_ok_sub in Hcall; try assumption;
+             apply call_ok_sym in Hcall; try assumption;
+             repeat apply call_ok_sub in Hcall; try assumption;
+             apply call_ok_sym; try assumption
+      | [ Hspawn : spawn_ok _ _ _ _ _ _ |- spawn_ok _ _ _ _ _ _ ]
+          => repeat apply spawn_ok_sub in Hspawn; try assumption;
+             apply spawn_ok_sym in Hspawn; try assumption;
+             repeat apply spawn_ok_sub in Hspawn; try assumption;
+             apply spawn_ok_sym; try assumption
+      end.
+
+Theorem ni : NIWeak' PAYD COMPT COMPTDEC COMPS IENVD KSTD INIT HANDLERS labeler.
+Proof.
+  apply ni_suf.
+  unfold NonInterferenceSt'.
+  intros.
+  inversion H1.
+  inversion H2.
+  intros.
+  destruct_msg.
+  repeat unpack.
+  simpl in *.
+  rewrite H in *.
+  inversion H7.
+  f_equal; auto.
+  apply H0; auto; try spawn_call.
+
+  unfold NonInterferenceSt'.
+  intros.
+  inversion H1.
+  destruct_msg.
+  repeat unpack.
+  simpl in *.
+  rewrite H in *.
+  apply H0; auto; try spawn_call.
+Qed.
+(*
+unfold NIWeak'.
+unfold NonInterference'.
+  unfold NonInterferenceSt'.
+  intros.
+  generalize dependent tr1.
+  generalize dependent tr2.
+  generalize dependent s2.
+  induction H; intros.
+    induction H0.
+      admit.
+
+      inversion H6.
+      destruct_msg.
+      repeat unpack.
+      simpl in *.
+      destruct (labeler c).
+        admit.
+        admit.
+
+      admit.
+
+    inversion H0.
+    destruct_msg.
+    repeat unpack.
+    simpl in *.
+    destruct (labeler c).
+      simpl in *.
+      apply call_ok_sym in H4.
+      repeat apply call_ok_sub in H4.
+      apply spawn_ok_sym in H5.
+      repeat apply spawn_ok_sub in H5.
+      generalize dependent tr2.
+      induction H1; intros.
+        admit.
+
+        inversion H2.
+        destruct_msg.
+        repeat unpack.
+        simpl in *.
+        destruct (labeler c0).
+          inversion H6.
+          replace a with a0 in * by admit.
+          replace b with b0 in * by admit.
+          f_equal; auto.
+          apply IHReach with (s2:=s1); auto.
+          admit.
+          admit.
+
+          apply IHReach0; auto.
+          admit.
+          admit.
+
+        subst s'.
+        simpl in *.
+        apply pack_injective in H4.
+        subst tr2.
+        simpl in *.
+        apply IHReach0; auto.
+        admit.
+        admit.
+
+    apply IHReach with (s2:=s2); auto.
+admit.
+admit.
+
+apply
+  inversion H0.
+  inversion H1.
+  destruct_msg.
+  repeat unpack.
+  simpl in *.
+  destruct (labeler c).
+  
+    
+
+  apply H; eauto.
+  apply call_ok_sym in H3; apply call_ok_sym;
+  repeat apply call_ok_sub in H3; assumption.
+  apply spawn_ok_sym in H4; apply spawn_ok_sym;
+  repeat apply spawn_ok_sub in H4; assumption.
+Qed.
+*)
 End Spec.
 
 Module Main := MkMain(Spec).
