compiler/dsl/coq/NonInterference.v
@@ -1,0 +1,652 @@
+Require Import Reflex.
+Require Import ReflexBase.
+Require Import List.
+Require Import Ynot.
+
+Section NI.
+
+Context {NB_MSG : nat}.
+Variable PAYD     : vvdesc NB_MSG.
+Variable COMPT    : Set.
+Variable COMPTDEC : forall (x y : COMPT), decide (x = y).
+Variable COMPS    : COMPT -> compd.
+Variable IENVD    : vcdesc COMPT.
+Variable KSTD     : vcdesc COMPT.
+Variable INIT : init_prog PAYD COMPT COMPS KSTD IENVD.
+Variable HANDLERS : handlers PAYD COMPT COMPS KSTD.
+Definition comp := comp COMPT COMPS.
+Definition Reach := Reach PAYD COMPT COMPTDEC COMPS KSTD IENVD INIT HANDLERS.
+Definition KTrace := KTrace PAYD COMPT COMPS.
+Definition KAction := KAction PAYD COMPT COMPS.
+Definition kstate := kstate PAYD COMPT COMPS KSTD.
+
+Definition is_input labeler (act : KAction) :=
+  match act with
+  | KRecv c _ => labeler c
+  | KBogus c _ => labeler c
+  | _        => false
+  end.
+
+Definition is_output labeler (act : KAction) :=
+  match act with
+  | KSend c _   => labeler c
+  | KExec _ _ c => labeler c
+  | _           => false
+  end.
+
+Definition inputs labeler (tr : KTrace) :=
+  filter (is_input labeler) tr.
+
+Definition outputs labeler (tr : KTrace) :=
+  filter (is_output labeler) tr.
+
+Definition KCall := KCall PAYD COMPT COMPS.
+Definition KExec := KExec PAYD COMPT COMPS.
+Definition KRecv := KRecv PAYD COMPT COMPS.
+
+Definition call_ok nd_filt (tr1 : KTrace) (tr2 : KTrace) :=
+  forall prog args f1 f2 tr1bef tr1aft tr2bef tr2aft,
+    tr1 = tr1aft ++ (KCall prog args f1::tr1bef) ->
+    tr2 = tr2aft ++ (KCall prog args f2::tr2bef) ->
+    filter nd_filt tr1bef = filter nd_filt tr2bef ->
+    f1 = f2.
+
+Definition spawn_ok nd_filt (tr1 : KTrace) (tr2 : KTrace) :=
+  forall prog args c1 c2 tr1bef tr1aft tr2bef tr2aft,
+    tr1 = tr1aft ++ (KExec prog args c1::tr1bef) ->
+    tr2 = tr2aft ++ (KExec prog args c2::tr2bef) ->
+    filter nd_filt tr1bef = filter nd_filt tr2bef ->
+    (comp_fd _ _ c1) = (comp_fd _ _ c2).
+
+Definition NonInterferenceSt' nd_filt labeler (s1 s2:kstate) : Prop :=
+  forall tr1 tr2, ktr _ _ _ _ s1 = [tr1]%inhabited ->
+                  ktr _ _ _ _ s2 = [tr2]%inhabited ->
+                  call_ok nd_filt tr1 tr2 ->
+                  spawn_ok nd_filt tr1 tr2 ->
+                  inputs labeler tr1 = inputs labeler tr2 ->
+                  outputs labeler tr1 = outputs labeler tr2.
+
+Definition NonInterference' nd_filt labeler : Prop :=
+  forall s1 s2, Reach s1 -> Reach s2 ->
+                NonInterferenceSt' nd_filt labeler s1 s2.
+
+Definition NonInterference nd_filt labeler : Prop :=
+  forall s1 s2 tr1 tr2, Reach s1 -> Reach s2 ->
+                        ktr _ _ _ _ s1 = [tr1]%inhabited ->
+                        ktr _ _ _ _ s2 = [tr2]%inhabited ->
+                        call_ok nd_filt tr1 tr2 ->
+                        spawn_ok nd_filt tr1 tr2 ->
+                        inputs labeler tr1 = inputs labeler tr2 ->
+                        outputs labeler tr1 = outputs labeler tr2.
+
+Definition nd_weak : KAction -> bool := fun _ => false.
+
+(*Non deterministic calls are independent of the trace history.*)
+Definition NIWeak := NonInterference nd_weak.
+Definition NIWeak' := NonInterference' nd_weak.
+
+Lemma call_ok_sub : forall nd_filt act tr1 tr2,
+  call_ok nd_filt tr1 (act::tr2) ->
+  call_ok nd_filt tr1 tr2.
+Proof.
+  unfold call_ok; intros.
+  apply H with (prog:=prog) (args:=args) (tr1bef:=tr1bef) (tr2bef:=tr2bef)
+               (tr1aft:=tr1aft) (tr2aft:=(act::tr2aft)); subst tr2; auto.
+Qed.
+
+Lemma spawn_ok_sub : forall nd_filt act tr1 tr2,
+  spawn_ok nd_filt tr1 (act::tr2) ->
+  spawn_ok nd_filt tr1 tr2.
+Proof.
+  unfold spawn_ok; intros.
+  apply H with (prog:=prog) (args:=args) (tr1bef:=tr1bef) (tr2bef:=tr2bef)
+               (tr1aft:=tr1aft) (tr2aft:=(act::tr2aft)); subst tr2; auto.
+Qed.
+
+Lemma call_ok_sym : forall nd_filt tr1 tr2,
+  call_ok nd_filt tr1 tr2 ->
+  call_ok nd_filt tr2 tr1.
+Proof.
+  unfold call_ok; intros.
+  symmetry.
+  eauto.
+Qed.
+
+Lemma spawn_ok_sym : forall nd_filt tr1 tr2,
+  spawn_ok nd_filt tr1 tr2 ->
+  spawn_ok nd_filt tr2 tr1.
+Proof.
+  unfold spawn_ok; intros.
+  symmetry.
+  eauto.
+Qed.
+
+Hint Resolve call_ok_sub spawn_ok_sub call_ok_sym spawn_ok_sym.
+
+Lemma nist_sym : forall s1 s2 nd_filt lblr,
+  NonInterferenceSt' nd_filt lblr s1 s2 ->
+  NonInterferenceSt' nd_filt lblr s2 s1.
+Proof.
+  unfold NonInterferenceSt'.
+  intros.
+  symmetry.
+  apply H; auto.
+Qed.
+
+Lemma init_tr_same : forall s1 s2 tr1 tr2,
+  InitialState PAYD COMPT COMPTDEC COMPS KSTD IENVD INIT s1 ->
+  InitialState PAYD COMPT COMPTDEC COMPS KSTD IENVD INIT s2 ->
+  ktr _ _ _ _ s1 = [tr1]%inhabited ->
+  ktr _ _ _ _ s2 = [tr2]%inhabited ->
+  tr1 = tr2.
+Proof.
+  intros s1 s2 tr1 tr2 HI1 HI2 Htr1 Htr2.
+  destruct HI1 as [ s1' Hs1' _].
+  destruct HI2 as [s2' Hs2' _].
+  subst s1'.
+  subst s2'.
+  apply pack_injective.
+  rewrite <- Htr1.
+  rewrite <- Htr2.
+  reflexivity.
+Qed.
+
+Lemma init_inputs_nil : forall s tr lblr,
+  InitialState PAYD COMPT COMPTDEC COMPS KSTD IENVD INIT s ->
+  ktr _ _ _ _ s = [tr]%inhabited ->
+  inputs lblr tr = nil.
+Proof.
+  intros s tr lblr HInit Htr;
+  destruct HInit; subst s;
+  generalize dependent tr.
+  case_eq (init_ktr _ _ _ _ _ (initial_init_state PAYD COMPT COMPS KSTD IENVD)).
+  intros k Htri.
+  assert (inputs lblr k = nil) by
+      (simpl in Htri; apply pack_injective in Htri; rewrite <- Htri; auto).
+  generalize dependent k.
+  generalize dependent (initial_init_state PAYD COMPT COMPS KSTD IENVD).
+  induction INIT; intros ist k Htri H tr Htr; simpl in *;
+    try (destruct ist; destruct init_ktr as [k']; simpl in *;
+    apply pack_injective in Htr; subst tr; apply pack_injective in Htri;
+    subst k'; auto).
+
+    case_eq (init_ktr _ _ _ _ _
+               (init_state_run_cmd PAYD COMPT COMPTDEC COMPS KSTD IENVD ist i1));
+    intros.
+    apply IHi2 with
+      (i:=(init_state_run_cmd PAYD COMPT COMPTDEC COMPS KSTD IENVD ist i1))
+      (k:=k0); auto.
+    apply IHi1 with (i:=ist) (k:=k); auto.
+    destruct ist; auto.
+
+    destruct ist;
+    match goal with
+    | [ _ : context[if ?e then _ else _] |- _ ]
+        => destruct e
+    end; eauto.
+
+    (*Send all*)
+    induction init_comps; auto; simpl;
+      match goal with
+      |- context[ if ?e then _ else _ ]
+         => destruct e
+      end; auto.
+Qed.
+
+Lemma hdlr_no_recv :
+  forall c m envd (hst:hdlr_state PAYD COMPT COMPS KSTD envd) stmt tr tr' lblr,
+  ktr _ _ _ _ (hdlr_kst _ _ _ _ _ hst) = [tr]%inhabited ->
+  ktr _ _ _ _ (hdlr_kst _ _ _ _ _
+    (hdlr_state_run_cmd _ _ COMPTDEC _ _ c m _ hst stmt))
+  = [tr']%inhabited ->
+  exists tr'', tr' = tr'' ++ tr /\
+               forall act, In act tr'' ->
+                           is_input lblr act = false.
+Proof.
+  intros.
+  generalize dependent hst.
+  generalize dependent tr.
+  generalize dependent tr'.
+  induction stmt; intros tr' tr hst.
+    destruct hst as [hkst henv];
+    destruct hkst; intros; simpl in *.
+    exists nil.
+    rewrite H in H0.
+    apply pack_injective in H0.
+    split; auto.
+    intros.
+    simpl in *.
+    contradiction.
+
+    intros.
+    case_eq (ktr PAYD COMPT COMPS KSTD
+              (hdlr_kst PAYD COMPT COMPS KSTD envd
+                 (hdlr_state_run_cmd PAYD COMPT COMPTDEC COMPS KSTD c m envd
+                    hst stmt1))); intros.
+    pose proof (IHstmt1 k tr hst H H1).
+    pose (hst1:=hdlr_state_run_cmd PAYD COMPT COMPTDEC COMPS KSTD c m envd
+                    hst stmt1).
+    destruct hst as [hkst henv].
+    destruct hkst.
+    pose proof (IHstmt2 tr' k hst1 H1 H0).
+    destruct H2.
+    destruct H2.
+    destruct H3.
+    destruct H3.
+    exists (x0++x).
+    split.
+      subst tr'.
+      subst k.
+      symmetry.
+      apply app_ass.
+
+      intros.
+      apply in_app_or in H6.
+      destruct H6.
+      apply H5; auto.
+      apply H4; auto.
+
+    intros.
+    destruct hst as [hkst henv]_eqn.
+    destruct hkst.
+    simpl in *.
+    match goal with
+    | [ _ : context[if ?e then _ else _] |- _ ]
+      => destruct e
+    end; [apply IHstmt2 with (hst:=hst) | apply IHstmt1 with (hst:=hst)];
+    subst hst; auto.
+
+    intros.
+    destruct hst as [hkst henv];
+    destruct hkst; intros; simpl in *.
+    destruct ktr.
+    simpl in *.
+    apply pack_injective in H0.
+    subst tr'.
+    apply pack_injective in H.
+    subst k.
+    match goal with
+    |- exists _, (?act::_) = _ ++ _ /\ _
+      => exists (act::nil)
+    end.
+    split; auto.
+    intros.
+    simpl in *.
+    destruct H.
+      subst act; auto.
+      contradiction.
+
+    intros.
+    destruct hst as [hkst henv].
+    destruct hkst.
+    generalize dependent tr'.
+    induction kcs; intros.
+      destruct ktr; simpl in *.
+      exists nil.
+      apply pack_injective in H; subst tr.
+      apply pack_injective in H0; subst tr'.
+      split; auto.
+      intros; simpl in *; contradiction.
+
+      simpl in *.
+      match goal with
+      | [ _ : context[ if ?e then _ else _ ] |- _ ]
+          => destruct e
+      end; try solve [apply IHkcs; auto].
+      destruct ktr.
+      simpl in *.
+      apply pack_injective in H0; subst tr'.
+      match goal with
+      | [ _ : _ -> forall _, [?tr0]%inhabited = _ -> _ |- _ ]
+          => pose proof (IHkcs H tr0 (Logic.eq_refl [tr0]%inhabited))
+      end.
+      destruct H0.
+      exists (KSend PAYD COMPT COMPS a
+       {|
+       tag := t;
+       pay := eval_hdlr_payload_expr PAYD COMPT COMPS KSTD c m envd kst henv
+                (lkup_tag PAYD t) p |}::x).
+      destruct H0.
+      split.
+        rewrite <- app_comm_cons.
+        f_equal.
+        assumption.
+
+        intros.
+        simpl in *.
+        destruct H2; auto.
+        subst act; auto.
+
+    intros.
+    destruct hst as [hkst henv];
+    destruct hkst; intros; simpl in *.
+    destruct ktr.
+    simpl in *.
+    apply pack_injective in H0.
+    subst tr'.
+    apply pack_injective in H.
+    subst k.
+    match goal with
+    |- exists _, (?act::_) = _ ++ _ /\ _
+      => exists (act::nil)
+    end.
+    split; auto.
+    intros.
+    simpl in *.
+    destruct H.
+      subst act; auto.
+      contradiction.
+
+    intros.
+    destruct hst as [hkst henv];
+    destruct hkst; intros; simpl in *.
+    destruct ktr.
+    simpl in *.
+    apply pack_injective in H0.
+    subst tr'.
+    apply pack_injective in H.
+    subst k.
+    exists nil.
+    split; auto.
+    intros.
+    simpl in *.
+    contradiction.
+Qed.      
+
+
+Lemma ve_inputs_high : forall c m s s' tr tr' lblr,
+  lblr c = true ->
+  ktr _ _ _ _ s = [tr]%inhabited ->
+  ktr _ _ _ _ s' = [tr']%inhabited ->
+  ValidExchange PAYD COMPT COMPTDEC COMPS KSTD HANDLERS c m s s' ->
+  inputs lblr tr' = KRecv c m :: (inputs lblr tr).
+Proof.
+  intros c m s s' tr tr' lblr Hhigh Htr Htr' Hve.
+  inversion Hve.
+  unfold kstate_run_prog in H2.
+  apply f_equal with (f:=ktr PAYD COMPT COMPS KSTD) in H0.
+  simpl in H0.
+  match goal with
+  | [ _ : hdlr_kst _ _ _ _ ?envd
+                   (hdlr_state_run_cmd _ _ _ _ _ ?c ?m _ ?hst ?stmt) = _,
+      Hmid : ktr _ _ _ _ _ = [?trmid]%inhabited |- _ ]
+    => pose proof (hdlr_no_recv c m envd hst stmt trmid tr' lblr Hmid)
+  end.
+  subst s'.
+  apply H3 in Htr'.
+  destruct Htr'.
+  destruct H2.
+  subst tr'.
+  match goal with
+  |- inputs ?lblr (?x++?act1::?act2::?tr0) = _
+    => replace (inputs lblr (x++act1::act2::tr0)) with
+       (inputs lblr (act1::act2::tr0))
+  end.
+  simpl.
+  rewrite H in Htr.
+  apply pack_injective in Htr.
+  subst tr.
+  rewrite Hhigh.
+  auto.
+  clear H3.
+  induction x.
+    auto.
+
+    simpl in *.
+    rewrite Hhigh in *.
+    pose proof (H4 a).
+    simpl in H2.
+    pose proof (H2 (or_introl _ (Logic.eq_refl a))).
+    rewrite H3.
+    apply IHx; auto.
+Qed.
+
+Lemma ve_inputs_low : forall c m s s' tr tr' lblr,
+  lblr c = false ->
+  ktr _ _ _ _ s = [tr]%inhabited ->
+  ktr _ _ _ _ s' = [tr']%inhabited ->
+  ValidExchange PAYD COMPT COMPTDEC COMPS KSTD HANDLERS c m s s' ->
+  inputs lblr tr' = inputs lblr tr.
+Proof.
+  intros c m s s' tr tr' lblr Hhigh Htr Htr' Hve.
+  inversion Hve.
+  unfold kstate_run_prog in H2.
+  apply f_equal with (f:=ktr PAYD COMPT COMPS KSTD) in H0.
+  simpl in H0.
+  match goal with
+  | [ _ : hdlr_kst _ _ _ _ ?envd
+                   (hdlr_state_run_cmd _ _ _ _ _ ?c ?m _ ?hst ?stmt) = _,
+      Hmid : ktr _ _ _ _ _ = [?trmid]%inhabited |- _ ]
+    => pose proof (hdlr_no_recv c m envd hst stmt trmid tr' lblr Hmid)
+  end.
+  subst s'.
+  apply H3 in Htr'.
+  destruct Htr'.
+  destruct H2.
+  subst tr'.
+  match goal with
+  |- inputs ?lblr (?x++?act1::?act2::?tr0) = _
+    => replace (inputs lblr (x++act1::act2::tr0)) with
+       (inputs lblr tr0)
+  end.
+  rewrite H in Htr.
+  apply pack_injective in Htr.
+  subst tr.
+  auto.
+
+  induction x.
+    simpl.
+    rewrite Hhigh.
+    auto.
+
+    simpl in *.
+    pose proof (H4 a).
+    simpl in H2.
+    pose proof (H2 (or_introl _ (Logic.eq_refl a))).
+    rewrite H5.
+    apply IHx; eauto.
+Qed.    
+
+Ltac high_ins :=
+  match goal with
+  | [ ce : Reflex.comp _ _, me : msg _ |- _]
+      => match goal with
+         | [ _ : ValidExchange _ _ _ _ _ _ ce me ?sb ?sa,
+             _ : ktr _ _ _ _ ?sa = [?tra]%inhabited,
+             Hin : context[inputs _ ?tra] |- _ ]
+             => let cs := fresh "cs" in
+                let itr := fresh "itr" in
+                let trb := fresh "tr" in
+                let st := fresh "st" in
+                let fd := fresh "fd" in
+                destruct sb as [cs itr st fd]_eqn; destruct itr as [trb];
+                rewrite ve_inputs_high with (c:=ce) (m:=me) (s:=sb) (s':=sa) (tr:=trb) (tr':=tra) in Hin;
+                subst sb; auto
+         end
+  end.
+
+Ltac low_ins :=
+  match goal with
+  | [ ce : Reflex.comp _ _, me : msg _ |- _]
+      => match goal with
+         | [ _ : ValidExchange _ _ _ _ _ _ ce me ?sb ?sa,
+             _ : ktr _ _ _ _ ?sa = [?tra]%inhabited,
+             Hin : context[inputs _ ?tra] |- _ ]
+             => let cs := fresh "cs" in
+                let itr := fresh "itr" in
+                let trb := fresh "tr" in
+                let st := fresh "st" in
+                let fd := fresh "fd" in
+                destruct sb as [cs itr st fd]_eqn; destruct itr as [trb];
+                rewrite ve_inputs_low with (c:=ce) (m:=me) (s:=sb) (s':=sa) (tr:=trb) (tr':=tra) in Hin;
+                subst sb; auto
+         end
+  end.
+
+Theorem ni_suf : forall lblr nd_filt,
+  (forall c m s1 s1' s2 s2',
+     lblr c = true ->
+     NonInterferenceSt' nd_filt lblr s1 s2 ->
+     ValidExchange PAYD COMPT COMPTDEC COMPS KSTD HANDLERS c m s1 s1' ->
+     ValidExchange PAYD COMPT COMPTDEC COMPS KSTD HANDLERS c m s2 s2' ->
+     NonInterferenceSt' nd_filt lblr s1' s2') ->
+  (forall c m s1 s1' s2,
+     lblr c = false ->
+     NonInterferenceSt' nd_filt lblr s1 s2 ->
+     ValidExchange PAYD COMPT COMPTDEC COMPS KSTD HANDLERS c m s1 s1' ->
+     NonInterferenceSt' nd_filt lblr s1' s2) ->
+  NonInterference' nd_filt lblr.
+Proof.
+  unfold NonInterference'.
+  intros.
+  generalize dependent s2.
+  induction H1; intros.
+    induction H2.
+      unfold NonInterferenceSt'; intros.
+      assert (tr1 = tr2) as Heq by (apply init_tr_same with (s1:=s) (s2:=s0); auto).
+      rewrite Heq.
+      reflexivity.
+
+      case_eq (lblr c); intros.
+        unfold NonInterferenceSt'.
+        intros.
+        assert (inputs lblr tr1 = nil) as Heq by
+          (apply init_inputs_nil with (s:=s); auto).
+        rewrite Heq in H9.
+        high_ins.
+        discriminate.
+
+        apply nist_sym.
+        apply nist_sym in IHReach.
+        apply H0 with (c:=c) (m:=m) (s1:=s0); auto.
+
+      rewrite H4.
+      unfold NonInterferenceSt'.
+      simpl.
+      intros.
+      apply pack_injective in H6.
+      subst tr2.
+      simpl in *.
+      unfold NonInterferenceSt' in IHReach.
+      simpl in IHReach.
+      destruct (lblr f).
+        assert (inputs lblr tr1 = nil) as Heq by
+          (apply init_inputs_nil with (s:=s); auto).
+        rewrite Heq in H9.
+        discriminate.
+      
+        apply IHReach; auto.
+          repeat apply call_ok_sub in H7; assumption.
+          repeat apply spawn_ok_sub in H8; assumption.
+
+    case_eq (lblr c); intros.    
+      induction H3.
+        unfold NonInterferenceSt'; intros.
+        assert (inputs lblr tr2 = nil) as Heq by
+          (apply init_inputs_nil with (s:=s0); auto).
+        rewrite Heq in H9.
+        high_ins.
+        discriminate.
+
+        case_eq (lblr c0); intros.
+          unfold NonInterferenceSt'; intros.
+          assert (c0 = c) by (repeat high_ins; inversion H11; auto).
+          assert (m0 = m) by (repeat high_ins; inversion H11; auto).
+          subst c0.
+          subst m0.
+          unfold NonInterferenceSt' at 2 in H.
+          apply H with (m:=m) (c:=c) (s1:=s) (s1':=s') (s2:=s0) (s2':=s'0); auto.
+
+          apply nist_sym.
+          apply nist_sym in IHReach0.
+          apply H0 with (c:=c0) (m:=m0) (s1:=s0) (s1':=s'0) (s2:=s'); auto.
+          
+        rewrite H6.
+        unfold NonInterferenceSt'.
+        simpl.
+        intros.
+        apply pack_injective in H8.
+        subst tr2.
+        simpl in *.
+        unfold NonInterferenceSt' in IHReach.
+        simpl in IHReach.
+        unfold NonInterferenceSt' in IHReach0.
+        destruct (lblr f).
+          high_ins.
+          discriminate.
+
+          apply IHReach0; auto.
+            repeat apply call_ok_sub in H9; assumption.
+            repeat apply spawn_ok_sub in H10; assumption.
+          
+      apply H0 with (c:=c) (m:=m) (s1:=s); auto.
+
+    rewrite H3.
+    unfold NonInterferenceSt'.
+    simpl.
+    intros.
+    apply pack_injective in H5.
+    subst tr1.
+    simpl in *.
+    case_eq (lblr f); intros.
+      rewrite H5 in *.
+      generalize dependent tr2.
+      induction H4; intros.
+        assert (inputs lblr tr2 = nil) as Heq by
+          (apply init_inputs_nil with (s:=s0); auto).
+        rewrite Heq in H9.
+        discriminate.
+
+        case_eq (lblr c); intros.
+          high_ins.
+          discriminate.
+
+          low_ins.
+          unfold NonInterferenceSt' in H0.
+          symmetry.
+          apply H0 with (c:=c) (m:=m) (s1:={| kcs := cs0; ktr := [tr0]; kst := st; kfd := fd |})
+                        (s1':=s'0) (s2:=s') (tr1:=tr2)
+                        (tr2:=KBogus PAYD COMPT COMPS f bmsg :: KSelect PAYD COMPT COMPS cs f :: tr); auto.
+          intros.
+          subst s'.
+          simpl in *.
+          apply pack_injective in H13.
+          subst tr3.
+          simpl.
+          symmetry.
+          eapply IHReach0; eauto.
+          apply pack_injective in H12.
+          subst tr1.
+          assumption.
+          subst s'; auto.
+          simpl.
+          rewrite H5 in *.
+          symmetry.
+          rewrite <- ve_inputs_low with (c:=c) (m:=m) (s:={| kcs := cs0; ktr := [tr0]; kst := st; kfd := fd |})
+                                     (s':=s'0) (tr:=tr0) (tr':=tr2) in H10; auto.
+
+          subst s'0.
+          simpl in *.
+          apply pack_injective in H8.
+          subst tr2.
+          simpl in *.
+          destruct (lblr f0).
+            inversion H11.
+            unfold NonInterferenceSt' in IHReach.
+            eapply IHReach; eauto.
+            repeat apply call_ok_sub in H9; apply call_ok_sym in H9;
+            repeat apply call_ok_sub in H9; apply call_ok_sym in H9; assumption.
+            repeat apply spawn_ok_sub in H10; apply spawn_ok_sym in H10;
+            repeat apply spawn_ok_sub in H10; apply spawn_ok_sym in H10; assumption.
+
+            eapply IHReach0; auto.
+            repeat apply call_ok_sub in H9. assumption.
+            repeat apply spawn_ok_sub in H10; assumption.
+          
+      rewrite H5 in *.
+      unfold NonInterferenceSt' in IHReach.
+      simpl in IHReach.
+      eapply IHReach; eauto.
+Qed.
+
+End NI.
